compiler/backend/proofs/stack_removeProofScript.sml
@@ -168,6 +168,7 @@ val good_syntax_inst_def = Define`
   (good_syntax_inst (Const n _) k ⇔ n < k) ∧
   (good_syntax_inst (Arith (Shift _ n r2 _)) k ⇔ r2 < k ∧ n < k) ∧
   (good_syntax_inst (Arith (Binop _ n r2 ri)) k ⇔ r2 < k ∧ n < k ∧ (case ri of Reg r1 => r1 < k | _ => T)) ∧
+  (good_syntax_inst (Arith (Div r1 r2 r3)) k ⇔ r1 < k ∧ r2 < k ∧ r3 < k) ∧
   (good_syntax_inst (Arith (AddCarry r1 r2 r3 r4)) k ⇔ r1 < k ∧ r2 < k ∧ r3 < k ∧ r4 < k) ∧
   (good_syntax_inst (Arith (LongMul r1 r2 r3 r4)) k ⇔ r1 < k ∧ r2 < k ∧ r3 < k ∧ r4 < k) ∧
   (good_syntax_inst (Arith (LongDiv r1 r2 r3 r4 r5)) k ⇔ r1 < k ∧ r2 < k ∧ r3 < k ∧ r4 < k ∧ r5 < k) ∧
